Get rid of BiContext; regoose a bit

new/golang/defn/interface.v
@@ -8,15 +8,14 @@ Context `{ffi_syntax}.
 Definition get (f : go_string) : val :=
   λ: "v",
     let: "v" := (match: "v" with SOME "v" => "v" | NONE => #() #() end) in
-    let: ("encoded_type_name", "val") := "v" in
+    let: ("pkg_type_name", "val") := "v" in
     (match: GlobalGet (#"method:"%go + "encoded_type_name" + #" "%go + #f) with
        InjL <> => #() #()
      | InjR "m" => "m"
      end) "val".
 
 Local Definition make_def (pkg_type_name : go_string * go_string): val :=
-  λ: "v", InjL (#((hex_encode pkg_type_name.1) ++ " "%go
-                 ++ hex_encode pkg_type_name.2), "v").
+  λ: "v", InjR (InjRV (#pkg_type_name.1, #pkg_type_name.2), "v").
 Program Definition make := unseal (_:seal (@make_def)). Obligation 1. by eexists. Qed.
 Definition make_unseal : make = _ := seal_eq _.
 
