new/code/github_com/mit_pdos/gokv/kv.v
@@ -14,14 +14,10 @@ Definition KvCput : go_type := interfaceT.
 
 Definition KvCput' : (go_string * go_string) := (pkg_name', "KvCput").
 
-Definition define' : val :=
-  rec: "define'" <> :=
-    exception_do (do:  #()).
-
 Definition initialize' : val :=
   rec: "initialize'" <> :=
     globals.package_init pkg_name' (λ: <>,
-      exception_do (do:  (define' #()))
+      exception_do (do:  #())
       ).
 
 End code.
